
> [!INFO] Inverse Function Theorem
> If $f$ is a differentiable function that is one-to-one near $a$ and $f'(a)\ne{0}$, then
> 		(a) $f^{-1}(x)$ is defined for $x$ near $b=f(a)$ (by definition of one-to-one)
> 		(b) $f^{-1}(x)$ is differentiable near $b=f(a)$
> 		(c) $\left[ \frac{d}{dx}f^{-1}(x) \right]_{x=b}=\frac{1}{f'(a)},$ where $b=f(a)\leftrightarrow f^{-1}(b)=a$
> 
> **In other words,**
> $$\frac{d}{dx}f^{-1}(x)=\frac{1}{f'(f^{-1}(x))}$$


### Related
---
- [[Derivative]]
- [[Derivative of Trigonometric Functions#Derivative of Inverse Trig]]
- 