Logarithms allow us to use addition in place of multiplication.

> [!INFO] The Main Point (Logarithmic Differentiation)
> $$\frac{d}{dx}\ln(f(x))=\frac{1}{f(x)}f'(x)=\frac{f'(x)}{f(x)}$$

> [!EXAMPLE] 
> $$f(x)=\frac{x^{9}e^4x}{\sqrt{ x-4 }}\to \ln(f(x))=\ln(x^9)+\ln(e^4x)-\ln(\sqrt{x-4})=9\ln x+4x-\frac{1}{2}\ln(x-4)$$
> 
> Differentiate:
> $$\frac{f'(x)}{f(x)}=\frac{9}{x}+4-\frac{1}{2}\cdot \frac{1}{x-4}\to f'(x)=\left( \frac{9}{x}+4-\frac{1}{2}\cdot \frac{1}{x-4} \right)\times\left( \frac{x^9e^4x}{\sqrt{ x-4 }} \right)$$



---
### Related
---
- [[Derivative]]